theories/lifting.v
@@ -1,0 +1,85 @@
+From machine_program_logic.program_logic Require Import machine weakestpre.
+From HypVeri Require Import lang.
+From iris.proofmode Require Import tactics.
+
+Section lifting.
+
+Lemma machine_mixin : MachineMixin terminated step.
+Proof.
+  refine {| mixin_terminated_stuck := terminated_stuck |}.
+Qed.
+
+Canonical Structure hyp_machine :=
+  Machine terminated step (Some scheduler) machine_mixin.
+
+Context `{_ : !irisG hyp_machine Σ}.
+
+Lemma sswp_lift_step_fupd {i E Φ} m1 :
+  machine.terminated m1 = false →
+  (∀ σ1 , ⌜scheduled σ1 i⌝ -∗  state_interp σ1 ={E,∅}=∗
+    ⌜reducible m1 σ1⌝ ∗
+    ∀ m2 σ2 , ⌜step m1 σ1 m2 σ2 ⌝ ={∅}=∗ ▷ |={∅,E}=>
+      state_interp σ2 ∗  Φ m2 )
+  ⊢ SSWP m1 @ i; E {{ Φ }}.
+Proof.
+  by rewrite sswp_eq /sswp_def=>->.
+Qed.
+
+Lemma sswp_lift_step {i E Φ} m1 :
+  machine.terminated m1 = false →
+  (∀ σ1 , ⌜scheduled σ1 i⌝ -∗  state_interp σ1 ={E,∅}=∗
+    ⌜reducible m1 σ1⌝ ∗
+    ▷∀ m2 σ2 , ⌜step m1 σ1 m2 σ2 ⌝ ={∅,E}=∗
+      state_interp σ2 ∗  Φ m2 )
+  ⊢ SSWP m1 @ i; E {{ Φ }}.
+Proof.
+  iIntros (?) "H".
+  iApply sswp_lift_step_fupd; [done |].
+  iIntros (?) "Hsche Hσ".
+  iMod ("H" $! σ1 with "Hsche Hσ") as "[ $ H]".
+  iIntros "!> * % !> !>".
+  by iApply "H".
+Qed.
+
+
+Lemma sswp_lift_atomic_step_fupd {i E1 E2 Φ} m1 :
+  machine.terminated m1 = false →
+  (∀ σ1 , ⌜scheduled σ1 i⌝ -∗  state_interp σ1 ={E1}=∗
+    ⌜reducible m1 σ1⌝ ∗
+    ∀ m2 σ2 , ⌜step m1 σ1 m2 σ2 ⌝ ={E1} [E2]▷=∗
+      state_interp σ2 ∗  Φ m2 )
+  ⊢ SSWP m1 @ i; E1 {{ Φ }}.
+Proof.
+  iIntros (?) "H".
+  iApply (sswp_lift_step_fupd m1)=>//.
+  iIntros (?) "Hsche Hσ".
+  iMod ("H" $! σ1 with "Hsche Hσ") as "[$ H]".
+  iApply fupd_mask_intro;first set_solver.
+  iIntros "Hclose" (m2 σ2 ?).
+  iMod "Hclose" as "_".
+  iMod ("H" $! m2 σ2 with "[#]") as "H";[done|].
+  iApply fupd_mask_intro;first set_solver.
+  iIntros " Hclose !>".
+  iMod "Hclose" as "_".
+  by iApply "H".
+Qed.
+
+Lemma sswp_lift_atomic_step {i E Φ} m1 :
+  machine.terminated m1 = false →
+  (∀ σ1 , ⌜scheduled σ1 i⌝ -∗  state_interp σ1 ={E}=∗
+    ⌜reducible m1 σ1⌝ ∗
+    ▷ ∀ m2 σ2 , ⌜step m1 σ1 m2 σ2 ⌝ ={E}=∗
+      state_interp σ2 ∗  Φ m2 )
+  ⊢ SSWP m1 @ i; E {{ Φ }}.
+Proof.
+  iIntros (?) "H".
+  iApply (@sswp_lift_atomic_step_fupd i E E Φ);[done|].
+  iIntros (??) "Hσ".
+  iMod ("H" $! σ1 H0 with "Hσ") as "[$ H]".
+  iIntros "!> *".
+  iIntros (Hstep).
+  do 2 iModIntro.
+  by iApply "H".
+Qed.
+
+End lifting.
