theories/rule_base.v
@@ -1,0 +1,297 @@
+From iris.algebra Require Import gmap gset.
+From HypVeri Require Import RAs.
+
+  Lemma get_reg_gmap_lookup_Some σ i r w : (get_reg_gmap σ) !! (r,i)= Some w <->  get_vm_reg_file σ i !! r = Some w.
+    Proof.
+      split.
+      - unfold get_reg_gmap.
+        intro HSome.
+        apply elem_of_list_to_map_2 in HSome.
+        apply elem_of_list_In in HSome.
+        apply in_flat_map in HSome.
+        destruct HSome  as [i'] .
+        destruct H as [HiIn].
+        apply in_map_iff in H.
+        destruct H as [p].
+        destruct H as [Heqn].
+        inversion Heqn ;subst;clear Heqn.
+        apply elem_of_list_In in H.
+        by apply elem_of_map_to_list' in H.
+      - intro HSome.
+        apply  elem_of_list_to_map_1'.
+        + intros.
+          apply elem_of_list_In in H.
+          apply in_flat_map in H.
+          destruct H as [i'].
+          destruct H as [Hi'In H].
+          apply in_map_iff in H.
+          destruct H as [p].
+          destruct H as [Heqn H].
+          apply elem_of_list_In in H.
+          apply elem_of_map_to_list' in H.
+          inversion Heqn;subst;clear Heqn.
+          rewrite H in HSome.
+          by inversion HSome.
+        + apply elem_of_list_In.
+          apply in_flat_map.
+          exists i.
+          split;[apply in_list_of_vmids|].
+          apply in_map_iff.
+          exists (r,w).
+          split;[done|].
+          apply elem_of_list_In.
+          apply elem_of_map_to_list'.
+          done.
+    Qed.
+
+  Lemma get_reg_gmap_lookup_None σ i r : (get_reg_gmap σ) !! (r,i)= None <->  get_vm_reg_file σ i !! r = None.
+    Proof.
+      split.
+      - destruct (get_vm_reg_file σ i !! r) eqn:Heqn;[|done].
+        intro HNone.
+        apply not_elem_of_list_to_map_2 in HNone.
+        exfalso.
+        apply HNone.
+        apply elem_of_list_In.
+        apply in_map_iff.
+        exists (r,i,w).
+        split;[done|].
+        apply in_flat_map.
+        exists i.
+        split;[apply in_list_of_vmids|].
+        apply in_map_iff.
+        exists (r,w).
+        split;[done|].
+        apply elem_of_list_In.
+        apply elem_of_map_to_list'.
+        by simplify_eq /=.
+      - intro HNone.
+        apply  not_elem_of_list_to_map_1.
+        intro.
+        apply elem_of_list_In in H.
+          apply in_map_iff in H.
+          destruct H as [p].
+          destruct H as [Heqn H].
+          apply elem_of_list_In in H.
+          apply elem_of_list_In in H.
+          apply in_flat_map in H.
+          inversion Heqn;subst;clear Heqn.
+          destruct H as [i'].
+          destruct H as [HIn H].
+           apply in_map_iff in H.
+          destruct H as [p2].
+          destruct H as [Heqn H].
+          apply elem_of_list_In in H.
+          apply elem_of_map_to_list' in H.
+          inversion Heqn;subst;clear H0.
+          inversion H1;subst;clear H1.
+          rewrite H in HNone.
+          by inversion HNone.
+    Qed.
+
+
+  Lemma get_reg_gmap_get_vm_reg_file σ (r:reg_name) (i:vmid) :
+   (get_reg_gmap σ) !! (r,i) = (get_vm_reg_file σ i) !! r.
+    Proof.
+      destruct (get_reg_gmap σ !! (r, i)) eqn:Heqn.
+      apply get_reg_gmap_lookup_Some in Heqn;done.
+      apply get_reg_gmap_lookup_None in Heqn;done.
+    Qed.
+
+
+  Lemma get_reg_gmap_get_reg_Some σ (r:reg_name) (w:word) (i:vmid) : i= (get_current_vm σ)->
+                                                                   (get_reg_gmap σ) !! (r,i) = Some w <->
+                                                                   ((get_reg σ r) = Some w).
+  Proof.
+    intros.
+    rewrite get_reg_gmap_get_vm_reg_file.
+    unfold get_reg,get_reg_global;subst;done.
+  Qed.
+
+
+  Lemma update_reg_global_update_reg σ i r w : is_Some((get_reg_gmap σ) !! (r,i)) -> get_reg_gmap (update_reg_global σ i r w) =
+                                             <[(r,i) := w]>(get_reg_gmap σ).
+  Proof.
+    intros.
+    rewrite  /update_reg_global.
+    apply map_eq.
+    intro j.
+    destruct( decide (j=(r,i)) ).
+    - subst j.
+
+      rewrite lookup_insert.
+      rewrite get_reg_gmap_get_vm_reg_file.
+      rewrite /get_vm_reg_file /get_reg_files.
+        simpl.
+        rewrite -> (vlookup_insert i _  _).
+        by rewrite lookup_insert.
+    - destruct ((get_reg_gmap σ) !! j) eqn:Heqn;
+        rewrite lookup_insert_ne;[|done | |done];
+        rewrite -> Heqn;
+        destruct j as [r' i'];
+        rewrite ->get_reg_gmap_get_vm_reg_file in Heqn;
+        rewrite ->get_reg_gmap_get_vm_reg_file;
+        destruct (decide (i=i'));
+        destruct (decide (r=r'));
+        subst;
+        try contradiction;
+        rewrite - Heqn;
+        rewrite /get_vm_reg_file /get_reg_files;simpl.
+       + rewrite -> (vlookup_insert i' _ _).
+         by rewrite lookup_insert_ne ;[|done].
+       + by rewrite vlookup_insert_ne.
+       + by rewrite vlookup_insert_ne.
+       + rewrite -> (vlookup_insert i' _ _).
+         by rewrite lookup_insert_ne ;[|done].
+       + by rewrite vlookup_insert_ne ;[|done].
+       + by rewrite vlookup_insert_ne ;[|done].
+  Qed.
+
+  Lemma update_offset_PC_update_PC1 σ i (w:word) (o:nat):
+   i=get_current_vm σ -> ((get_reg_gmap σ) !! (PC,i) = Some w)
+   ->get_reg_gmap (update_offset_PC σ true o) = <[(PC,i) := (w +w o)]>(get_reg_gmap σ).
+  Proof.
+    intros.
+    rewrite /update_offset_PC.
+    remember H0.
+    clear Heqe.
+    rewrite /get_reg_gmap /update_reg_global in H0.
+    apply elem_of_list_to_map_2 in H0.
+    apply elem_of_list_In in H0.
+    apply in_flat_map in H0.
+    destruct H0.
+    destruct H0.
+    apply in_map_iff in H1.
+    destruct H1.
+    destruct H1.
+    inversion H1;subst;clear H1.
+    apply elem_of_list_In in H2.
+    apply elem_of_map_to_list' in H2.
+    rewrite H2.
+    rewrite /update_reg.
+    apply update_reg_global_update_reg.
+    exists x0.2.
+    by rewrite H4.
+  Qed.
+
+   Lemma update_reg_global_preserve_tx σ i r w : get_tx_agree (update_reg_global σ i r w) =
+                                               (get_tx_agree σ).
+  Proof.
+    rewrite /get_tx_agree /get_txrx_auth_agree.
+    f_equal.
+  Qed.
+
+  Lemma update_offset_PC_preserve_tx σ d o : get_tx_agree (update_offset_PC σ d o) = get_tx_agree σ.
+  Proof.
+    unfold update_offset_PC.
+    destruct (get_vm_reg_file σ (get_current_vm σ) !! PC).
+    destruct d; rewrite /update_reg update_reg_global_preserve_tx;done.
+    done.
+  Qed.
+
+ Lemma update_reg_global_preserve_rx1 σ i r w : get_rx_agree (update_reg_global σ i r w) =
+                                               (get_rx_agree σ).
+  Proof.
+    rewrite /get_rx_agree /get_txrx_auth_agree.
+    f_equal.
+  Qed.
+
+  Lemma update_offset_PC_preserve_rx1 σ d o : get_rx_agree (update_offset_PC σ d o) = get_rx_agree σ.
+  Proof.
+    unfold update_offset_PC.
+    destruct (get_vm_reg_file σ (get_current_vm σ) !! PC).
+    destruct d; rewrite /update_reg update_reg_global_preserve_rx1;done.
+    done.
+  Qed.
+
+
+   Lemma update_reg_global_preserve_rx2 σ i r w : get_rx_gmap (update_reg_global σ i r w) =
+                                               (get_rx_gmap σ).
+  Proof.
+    rewrite /get_rx_gmap /get_txrx_auth_agree.
+    f_equal.
+  Qed.
+
+  Lemma update_offset_PC_preserve_rx2 σ d o : get_rx_gmap (update_offset_PC σ d o) = get_rx_gmap σ.
+  Proof.
+    unfold update_offset_PC.
+    destruct (get_vm_reg_file σ (get_current_vm σ) !! PC).
+    destruct d; rewrite /update_reg update_reg_global_preserve_rx2;done.
+    done.
+  Qed.
+
+
+  (* TODO: the proofs above are identical *)
+
+  Lemma update_reg_global_preserve_rx σ i r w : (get_rx_agree (update_reg_global σ i r w), get_rx_gmap (update_reg_global σ i r w)) =
+                                               (get_rx_agree σ, get_rx_gmap σ).
+  Proof.
+    by rewrite update_reg_global_preserve_rx1 update_reg_global_preserve_rx2.
+  Qed.
+
+  Lemma update_offset_PC_preserve_rx  σ d o : (get_rx_agree (update_offset_PC σ d o), get_rx_gmap (update_offset_PC σ d o) ) =
+                                               (get_rx_agree σ, get_rx_gmap σ).
+  Proof.
+    by rewrite update_offset_PC_preserve_rx1 update_offset_PC_preserve_rx2 .
+  Qed.
+
+
+  Lemma update_reg_global_preserve_owned σ i r w : get_owned_gmap (update_reg_global σ i r w) =
+                                               (get_owned_gmap σ).
+  Proof.
+    rewrite /get_owned_gmap.
+    f_equal.
+    Qed.
+
+  Lemma update_offset_PC_preserve_owned σ d o : get_owned_gmap (update_offset_PC σ d o) = get_owned_gmap σ.
+  Proof.
+    unfold update_offset_PC.
+    destruct (get_vm_reg_file σ (get_current_vm σ) !! PC).
+    destruct d; rewrite /update_reg update_reg_global_preserve_owned;done.
+    done.
+  Qed.
+
+  Lemma update_reg_global_preserve_access σ i r w : get_access_gmap (update_reg_global σ i r w) =
+                                               (get_access_gmap σ).
+  Proof.
+    rewrite /get_access_gmap.
+    f_equal.
+    Qed.
+
+  Lemma update_offset_PC_preserve_access σ d o : get_access_gmap (update_offset_PC σ d o) = get_access_gmap σ.
+  Proof.
+    unfold update_offset_PC.
+    destruct (get_vm_reg_file σ (get_current_vm σ) !! PC).
+    destruct d; rewrite /update_reg update_reg_global_preserve_access;done.
+    done.
+  Qed.
+
+  Lemma update_reg_global_preserve_trans σ i r w : get_trans_gmap (update_reg_global σ i r w) =
+                                               (get_trans_gmap σ).
+  Proof.
+    rewrite /get_trans_gmap.
+    f_equal.
+  Qed.
+
+  Lemma update_offset_PC_preserve_trans σ d o : get_trans_gmap (update_offset_PC σ d o) = get_trans_gmap σ.
+  Proof.
+    unfold update_offset_PC.
+    destruct (get_vm_reg_file σ (get_current_vm σ) !! PC).
+    destruct d; rewrite /update_reg update_reg_global_preserve_trans;done.
+    done.
+  Qed.
+
+  Lemma update_reg_global_preserve_receivers σ i r w : get_receivers_gmap (update_reg_global σ i r w) =
+                                               (get_receivers_gmap σ).
+  Proof.
+    rewrite /get_receivers_gmap.
+    f_equal.
+  Qed.
+
+  Lemma update_offset_PC_preserve_receivers σ d o : get_receivers_gmap (update_offset_PC σ d o) = get_receivers_gmap σ.
+  Proof.
+    unfold update_offset_PC.
+    destruct (get_vm_reg_file σ (get_current_vm σ) !! PC).
+    destruct d; rewrite /update_reg update_reg_global_preserve_receivers;done.
+    done.
+  Qed.
